logicIntrinsic_subset_logicExtrinsic

NCML/IML/Semantics.lean
@@ -2,54 +2,54 @@ module
 
 public import NCML.Formula
 public import Mathlib.Order.Basic
-public import Mathlib.Tactic.Use
+public import Mathlib.Tactic
 
 @[expose] public section
 
-namespace NCML
+namespace NCML.IML
 
 variable {κ : Type*} [Nonempty κ]
 
-structure IMLKripkeFrame (κ : Type*) [Nonempty κ] where
+structure KripkeFrame (κ : Type*) [Nonempty κ] where
   iRel : κ → κ → Prop
   [iRel_paorder : IsPartialOrder _ iRel]
   mRel : κ → κ → Prop
 
-namespace IMLKripkeFrame
+namespace KripkeFrame
 
-abbrev World (_ : IMLKripkeFrame κ) := κ
+abbrev World (_ : KripkeFrame κ) := κ
 
-abbrev mRel' {F : IMLKripkeFrame κ} : F.World → F.World → Prop := F.mRel
-infixl:80 " ⊏ " => IMLKripkeFrame.mRel'
+abbrev mRel' {F : KripkeFrame κ} : F.World → F.World → Prop := F.mRel
+infixl:80 " ⊏ " => KripkeFrame.mRel'
 
-abbrev iRel' {F : IMLKripkeFrame κ} : F.World → F.World → Prop := F.iRel
-infixl:80 " ≼ " => IMLKripkeFrame.iRel'
+abbrev iRel' {F : KripkeFrame κ} : F.World → F.World → Prop := F.iRel
+infixl:80 " ≼ " => KripkeFrame.iRel'
 
-class MRelLifting (F : IMLKripkeFrame κ) where
-  mRel_lifting : ∀ {x₁ x₂ y₂ : F.World}, x₁ ≼ x₂ → x₂ ⊏ y₂ → ∃ y₁, y₁ ≼ y₂ ∧ x₁ ⊏ y₁
+class MRelLifting (F : KripkeFrame κ) where
+  mRel_lifting : ∀ x₁ x₂ y₂ : F.World, x₁ ≼ x₂ → x₂ ⊏ y₂ → ∃ y₁, y₁ ≼ y₂ ∧ x₁ ⊏ y₁
 export MRelLifting (mRel_lifting)
 
-class MixConfluent (F : IMLKripkeFrame κ) where
-  mix_confluent : ∀ {x₁ x₂ y₁ : F.World}, x₁ ≼ x₂ → x₁ ⊏ y₁ → ∃ y₂, y₁ ≼ y₂ ∧ x₂ ⊏ y₂
+class MixConfluent (F : KripkeFrame κ) where
+  mix_confluent : ∀ x₁ x₂ y₁ : F.World, x₁ ≼ x₂ → x₁ ⊏ y₁ → ∃ y₂, y₁ ≼ y₂ ∧ x₂ ⊏ y₂
 export MixConfluent (mix_confluent)
 
-end IMLKripkeFrame
+end KripkeFrame
 
 
-structure IMLKripkeModel (κ : Type*) [Nonempty κ] extends IMLKripkeFrame κ where
+structure KripkeModel (κ : Type*) [Nonempty κ] extends KripkeFrame κ where
   val : κ → Nat → Prop
-  val_persistent : ∀ {x₁ x₂ : toIMLKripkeFrame.World} {a}, val x₁ a → x₁ ≼ x₂ → val x₂ a
+  val_persistent : ∀ {x₁ x₂ : toKripkeFrame.World} {a}, val x₁ a → x₁ ≼ x₂ → val x₂ a
 
-namespace IMLKripkeModel
+namespace KripkeModel
 
-variable {M : IMLKripkeModel κ} {x₁ x₂ y₁ y₂ : M.World}
+variable {M : KripkeModel κ} {x₁ x₂ y₁ y₂ : M.World}
 variable {φ ψ : BDFormula}
 
 instance : IsPartialOrder M.World M.iRel := M.iRel_paorder
 instance : IsTrans M.World M.iRel := inferInstance
 
 @[grind]
-def ExtrinsicForces {M : IMLKripkeModel κ} (x₁ : M.World) : BDFormula → Prop
+def ExtrinsicForces {M : KripkeModel κ} (x₁ : M.World) : BDFormula → Prop
   | .atom a    => M.val x₁ a
   | .falsum    => False
   | .and φ ψ   => M.ExtrinsicForces x₁ φ ∧ M.ExtrinsicForces x₁ ψ
@@ -60,7 +60,7 @@ def ExtrinsicForces {M : IMLKripkeModel κ} (x₁ : M.World) : BDFormula → Pro
 infixl:80 " ⊩ᵉ " => ExtrinsicForces
 
 @[grind]
-def IntrinsicForces {M : IMLKripkeModel κ} (x₁ : M.World) : BDFormula → Prop
+def IntrinsicForces {M : KripkeModel κ} (x₁ : M.World) : BDFormula → Prop
   | .atom a    => M.val x₁ a
   | .falsum    => False
   | .and φ ψ   => M.IntrinsicForces x₁ φ ∧ M.IntrinsicForces x₁ ψ
@@ -96,7 +96,7 @@ lemma diaFree_formula_persistent_exrinsicForces [M.MRelLifting] (hφ : φ.diaFre
     apply h x₃ (Trans.trans Ix₁x₂ Ix₂x₃) hx₃φ;
   | box φ ihφ =>
     intro y₂ Mx₂y₂;
-    obtain ⟨y₁, Iy₁y₂, Mx₁y₁⟩ := M.mRel_lifting Ix₁x₂ Mx₂y₂;
+    obtain ⟨y₁, Iy₁y₂, Mx₁y₁⟩ := M.mRel_lifting _ _ _ Ix₁x₂ Mx₂y₂;
     apply ihφ (by grind) (h y₁ Mx₁y₁) Iy₁y₂;
 
 lemma boxFree_formula_persistent_exrinsicForces [M.MixConfluent] (hφ : φ.boxFree) : x₁ ⊩ᵉ φ → x₁ ≼ x₂ → x₂ ⊩ᵉ φ := by
@@ -109,14 +109,85 @@ lemma boxFree_formula_persistent_exrinsicForces [M.MixConfluent] (hφ : φ.boxFr
     apply h x₃ (Trans.trans Ix₁x₂ Ix₂x₃) hx₃φ;
   | dia φ ihφ =>
     obtain ⟨y₁, Mx₁y₁, hy₁⟩ := h;
-    obtain ⟨y₂, Iy₁y₂, My₁y₂⟩ := M.mix_confluent Ix₁x₂ Mx₁y₁;
+    obtain ⟨y₂, Iy₁y₂, My₁y₂⟩ := M.mix_confluent _ _ _ Ix₁x₂ Mx₁y₁;
     use y₂;
     constructor;
     . assumption;
     . exact ihφ (by grind) hy₁ Iy₁y₂;
 
-end IMLKripkeModel
+lemma formula_persistent_exrinsicForces [M.MRelLifting] [M.MixConfluent] : x₁ ⊩ᵉ φ → x₁ ≼ x₂ → x₂ ⊩ᵉ φ := by
+  intro h Ix₁x₂;
+  induction φ generalizing x₁ x₂ with
+  | atom a => apply M.val_persistent h Ix₁x₂;
+  | and | or | falsum => grind;
+  | imply φ ψ ihφ ihψ =>
+    intro x₃ Ix₂x₃ hx₃φ;
+    apply h x₃ (Trans.trans Ix₁x₂ Ix₂x₃) hx₃φ;
+  | box φ ihφ =>
+    intro y₂ Mx₂y₂;
+    obtain ⟨y₁, Iy₁y₂, Mx₁y₁⟩ := M.mRel_lifting _ _ _ Ix₁x₂ Mx₂y₂;
+    apply ihφ (h y₁ Mx₁y₁) Iy₁y₂;
+  | dia φ ihφ =>
+    obtain ⟨y₁, Mx₁y₁, hy₁⟩ := h;
+    obtain ⟨y₂, Iy₁y₂, My₁y₂⟩ := M.mix_confluent _ _ _ Ix₁x₂ Mx₁y₁;
+    use y₂;
+    constructor;
+    . assumption;
+    . exact ihφ hy₁ Iy₁y₂;
 
-end NCML
+
+def ExtrinsicValid (M : KripkeModel κ) (φ : BDFormula) := ∀ x : M.World, x ⊩ᵉ φ
+infixl:80 " ⊧ᵉ " => ExtrinsicValid
+
+def IntrinsicValid (M : KripkeModel κ) (φ : BDFormula) := ∀ x : M.World, x ⊩ᵉ φ
+infixl:80 " ⊧ⁱ " => IntrinsicValid
+
+end KripkeModel
+
+
+namespace KripkeFrame
+
+def ExtrinsicValid (F : KripkeFrame κ) (φ : BDFormula) := ∀ V hV, (KripkeModel.mk F V hV) ⊧ᵉ φ
+infixl:80 " ⊧ᵉ " => ExtrinsicValid
+
+def IntrinsicValid (F : KripkeFrame κ) (φ : BDFormula) := ∀ V hV, (KripkeModel.mk F V hV) ⊧ᵉ φ
+infixl:80 " ⊧ⁱ " => IntrinsicValid
+
+end KripkeFrame
+
+
+def logicExtrinsic := { φ : BDFormula | ∀ κ : Type*, [Nonempty κ] → ∀ M : KripkeModel κ, [M.MRelLifting] → [M.MixConfluent] → M ⊧ᵉ φ }
+def logicIntrinsic := { φ : BDFormula | ∀ κ : Type*, [Nonempty κ] → ∀ M : KripkeModel κ, M ⊧ⁱ φ }
+
+lemma wwwww {M : KripkeModel κ} [M.MRelLifting] [M.MixConfluent] {x₁ : M.World} {φ} : x₁ ⊩ᵉ φ ↔ x₁ ⊩ⁱ φ := by
+  induction φ generalizing x₁ with
+  | box φ ihφ =>
+    constructor;
+    . intro h y₁ Ix₁y₁ y₂ My₁y₂;
+      exact ihφ.mp $ KripkeModel.formula_persistent_exrinsicForces h Ix₁y₁ y₂ My₁y₂;
+    . intro h y₁ Mx₁y₁;
+      exact ihφ.mpr $ h x₁ (refl x₁) y₁ Mx₁y₁;
+  | dia φ ihφ =>
+    constructor;
+    . rintro ⟨y₁, Mx₁y₁, h⟩ x₂ Ix₁x₂;
+      obtain ⟨y₂, Iy₁y₂, Mx₁y₂⟩ := M.mix_confluent x₁ x₂ y₁ Ix₁x₂ Mx₁y₁;
+      use y₂;
+      constructor;
+      . assumption;
+      . exact ihφ.mp $ KripkeModel.formula_persistent_exrinsicForces h Iy₁y₂;
+    . rintro h;
+      obtain ⟨y₁, Mx₁y₁, h⟩ := h x₁ (refl _)
+      use y₁;
+      constructor;
+      . assumption;
+      . exact ihφ.mpr h;
+  | _ => grind;
+
+theorem logicIntrinsic_subset_logicExtrinsic : logicIntrinsic.{u} ⊆ logicExtrinsic.{u} := by
+  dsimp [logicIntrinsic, logicExtrinsic, KripkeModel.IntrinsicValid, KripkeModel.ExtrinsicValid];
+  grind [wwwww];
+
+
+end NCML.IML
 
 end
